Arithmetic: begin proofs of remaining weakening lemmas
- switch to MSets for exp_vars and stmt_vars functions
- fix _weakening_of_expression_semantics_3 statement:
    * requires the strong relation
    * now accounts for the isomorphism

Arithmetic/theories/Languages/MiniC/Lemmas.v
@@ -117,8 +117,8 @@ Proof with auto with rac_hint.
     pose proof (weakening_of_expression_semantics exp_sem Hext_exp) as exp_weak.
     unfold _weakening_of_statement_semantics_2 in Hext_stmt. 
     unfold _weakening_of_expression_semantics in Hext_exp.    
-    generalize dependent ev₀'.
-    induction Hderiv1 ; intros ev₀' Hrel ev₁' Hderiv2 ; inversion Hderiv2 ; subst ; try easy...
+    generalize dependent ev₀'. generalize dependent sub.
+    induction Hderiv1 ; intros sub ev₀' Hrel ev₁' Hderiv2 ; inversion Hderiv2 ; subst ; try easy...
 
     (* assign *)
     - split... simpl. intros v [Hnotin Hnotcompvar].  assert (HH: type_of_value (ev x) <> None) by congruence. apply type_of_value_env in HH.
@@ -137,7 +137,7 @@ Proof with auto with rac_hint.
             + now exists sub.
 
     (* seq *)
-    - admit.
+    - admit. 
     
     (* fcall *)
     - rewrite H9 in H0. inversion H0. subst. clear H0 H9 H8 H14. split ; admit.
@@ -162,96 +162,178 @@ Definition weakening_of_c_statements_semantics_2 {S T} :=
 
 
 Fact weakening_of_expression_semantics_3 {T : Set} : forall exp_sem, 
-    _weakening_of_expression_semantics_3 exp_sem exist_strong_env_mem_partial_order
-    -> _weakening_of_expression_semantics_3 (@generic_exp_sem T exp_sem) exist_strong_env_mem_partial_order
+    _weakening_of_expression_semantics_3 exp_sem strong_env_mem_partial_order
+    -> _weakening_of_expression_semantics_3 (@generic_exp_sem T exp_sem) strong_env_mem_partial_order
 .
-Proof with auto.
-    intros exp Hextweak ev e v Hderiv.
-    induction Hderiv; intros ev' [sub [Henv Hmem]] [HnotinEnv HnotinMem].
+Proof with eauto with rac_hint.
+    intros exp Hextweak ev e v sub Hderiv.
+    induction Hderiv; intros ev' Henvmem [HnotinEnv HnotinMem].
     - constructor.
     - assert (HxnotinEnv: ~ (dom ev - dom ev') x). {
         intros contra.  apply (HnotinEnv x contra); now left.
         }  
         apply not_in_sub_domain_prop in HxnotinEnv;[|apply in_domain_dec| apply in_domain_dec].
         constructor. destruct HxnotinEnv.
-        * destruct H0 as [z' Hevx]. specialize (Henv x _ _ Hevx). rewrite H in Henv. inversion Henv. 
+        * destruct H0 as [z' Hevx]. destruct Henvmem as [Henv _]. specialize (Henv x _ _ Hevx). rewrite H in Henv. inversion Henv. 
             destruct z' eqn:Z'Eqn.
             + destruct v eqn:VEqn.
                 ++ simpl in H1. inversion H1. now subst.
                 ++ destruct l; now subst.
             + simpl in H1. now subst.
         * exfalso. apply H0. now exists z. 
-    - admit.
-    - admit.
-    - admit.
-Admitted.
+    
+    - apply C_E_BinOpInt with z_ir z'_ir.
+        + apply IHHderiv1...
+            * split.
+                ** intros v Hdom. apply HnotinEnv in Hdom. simpl in Hdom. StringSet.D.fsetdec. 
+                ** intros.  apply HnotinMem in H0. destruct H0 as [x0 [Hevx0 HnotInx0]].
+                    exists x0. split... simpl in HnotInx0. StringSet.D.fsetdec.
+        + apply IHHderiv2...
+            * split.
+                ** intros v Hdom. apply HnotinEnv in Hdom. simpl in Hdom. 
+                    StringSet.D.fsetdec.
+                ** intros.  apply HnotinMem in H0. destruct H0 as [x0 [Hevx0 HnotInx0]].
+                    exists x0. split... simpl in HnotInx0. StringSet.D.fsetdec.
+
+    - eapply C_E_BinOpTrue...
+        + apply IHHderiv1...
+            * split.
+                ** intros v Hdom. apply HnotinEnv in Hdom. simpl in Hdom. StringSet.D.fsetdec.
+                ** intros.  apply HnotinMem in H0. destruct H0 as [x0 [Hevx0 HnotInx0]].
+                    exists x0. split... simpl in HnotInx0. StringSet.D.fsetdec.
+        + apply IHHderiv2...
+            * split.
+                ** intros v Hdom. apply HnotinEnv in Hdom. simpl in Hdom. StringSet.D.fsetdec.
+                ** intros. apply HnotinMem in H0. destruct H0 as [x0 [Hevx0 HnotInx0]].
+                    exists x0. split... simpl in HnotInx0. StringSet.D.fsetdec.
+
+    - eapply C_E_BinOpFalse...
+        + apply IHHderiv1...
+            * split.
+                ** intros v Hdom. apply HnotinEnv in Hdom. simpl in Hdom. StringSet.D.fsetdec.
+                ** intros.  apply HnotinMem in H0. destruct H0 as [x0 [Hevx0 HnotInx0]].
+                    exists x0. split... simpl in HnotInx0. StringSet.D.fsetdec.
+        + apply IHHderiv2...
+            * split.
+                ** intros v Hdom. apply HnotinEnv in Hdom. simpl in Hdom. StringSet.D.fsetdec.
+                ** intros.  apply HnotinMem in H0. destruct H0 as [x0 [Hevx0 HnotInx0]].
+                    exists x0. split... simpl in HnotInx0. StringSet.D.fsetdec.
+Qed.
 
 Definition weakening_of_c_expression_semantics_3 {T} := 
-    weakening_of_expression_semantics_3 (@Empty_exp_sem T) (weakening_of_empty_expression_semantics_3 exist_strong_env_mem_partial_order). 
+    weakening_of_expression_semantics_3 (@Empty_exp_sem T) (weakening_of_empty_expression_semantics_3 strong_env_mem_partial_order). 
 
 
 Lemma weakening_of_statement_semantics_3 {S T : Set} : 
     forall exp_sem stmt_sem ext_stmt_vars, 
-    _weakening_of_expression_semantics_3 exp_sem exist_strong_env_mem_partial_order
-    -> _weakening_of_statement_semantics_3 stmt_sem ext_stmt_vars  exist_strong_env_mem_partial_order
-    -> _weakening_of_statement_semantics_3 (@generic_stmt_sem S T exp_sem stmt_sem ext_stmt_vars) ext_stmt_vars exist_strong_env_mem_partial_order
+    _weakening_of_expression_semantics_3 exp_sem strong_env_mem_partial_order
+    -> _weakening_of_statement_semantics_3 stmt_sem ext_stmt_vars  strong_env_mem_partial_order
+    -> _weakening_of_statement_semantics_3 (@generic_stmt_sem S T exp_sem stmt_sem ext_stmt_vars) ext_stmt_vars strong_env_mem_partial_order
 .
 
-Proof with auto with rac_hint.
+Proof with eauto with rac_hint; try easy.
     intros exp_sem stmt_sem ext_stmt_vars ext_exp_weak ext_stmt_weak.
     epose proof (weakening_of_expression_semantics_3 exp_sem ext_exp_weak) as exp_weak.
-    intros f ev₀ s ev₁ Hderiv ev₀' Hrel [Henv Hmem].
+    intros f ev₀ s ev₁ sub Hderiv. 
 
-    induction Hderiv. 
+    induction Hderiv; intros ev₀' Hrel [Henv Hmem]. 
     (* skip *)
     - exists ev₀'. constructor.
 
     (* assign *)
     -  exists (ev₀' <| env ; vars ::= {{x\Def z}} |>). apply S_Assign...
-        +  apply env_same_ty with ev... left. pose proof strong_env_mem_stronger. destruct Hrel as [x0 Hrel]. exists x0. now apply H2. easy.
-        + apply weakening_of_expression_semantics_3 with ev... split. 
-            * intros v Hdom. apply Henv in Hdom. simpl in Hdom.  
-                apply Decidable.not_or in Hdom. now destruct Hdom.
-            * intros l Hdom. apply Hmem in Hdom as [l' Hdom]. simpl in Hdom.  exists l'. destruct Hdom. split... 
+        +  apply env_same_ty with ev... left. pose proof strong_env_mem_stronger. exists sub. now apply H2. 
+        + eapply weakening_of_expression_semantics_3... split. 
+            * intros v Hdom. apply Henv in Hdom. simpl in Hdom. StringSet.D.fsetdec.
+            * intros l Hdom. apply Hmem in Hdom as [l' Hdom]. simpl in Hdom. exists l'. destruct Hdom.  split...
+                StringSet.D.fsetdec. 
 
     (* if true *)
-    -  admit.
+    - destruct H as [He Hnotzero]. edestruct IHHderiv... 
+        * split. 
+            + intros v H. specialize (Henv v H). simpl in Henv. StringSet.D.fsetdec.
+            + intros x H. specialize (Hmem x H). simpl in Hmem.
+            destruct Hmem as [v [Hmpz Hmem]]. exists v. split... StringSet.D.fsetdec.
+        * exists x. apply S_IfTrue with z...
+            split... eapply weakening_of_expression_semantics_3... split.
+            + intros v Hdom. apply Henv in Hdom. simpl in Hdom. StringSet.D.fsetdec.
+            + intros l Hdom. apply Hmem in Hdom as [l' Hdom]. simpl in Hdom.  exists l'. destruct Hdom. split...
+                StringSet.D.fsetdec.
+
+
     (* if false *)
-    - admit.
+    - edestruct IHHderiv... 
+        * split. 
+            + intros v Hdom. specialize (Henv v Hdom). simpl in Henv. StringSet.D.fsetdec.
+            + intros x Hdom. specialize (Hmem x Hdom). simpl in Hmem.
+            destruct Hmem as [v [Hmpz Hmem]]. exists v. split... StringSet.D.fsetdec.
+
+        * exists x. apply S_IfFalse... eapply weakening_of_expression_semantics_3... split.
+            + intros v Hdom. apply Henv in Hdom. simpl in Hdom. StringSet.D.fsetdec. 
+            + intros l Hdom. apply Hmem in Hdom as [l' Hdom]. simpl in Hdom.  exists l'. destruct Hdom. split...
+                StringSet.D.fsetdec.
+
+
     (* while *)
-    - admit.
+    - edestruct IHHderiv... split.
+        *  intros v Hdom. specialize (Henv v Hdom). simpl in *. StringSet.D.fsetdec.
+        * intros x Hdom. specialize (Hmem x Hdom). simpl in Hmem.
+            destruct Hmem as [v [Hmpz Hmem]]. exists v. split...  simpl. StringSet.D.fsetdec.
+        
 
     (* seq *)
     - admit. 
 
     (* fcall *)
-    - eexists. apply S_FCall with b xargs zargs...
-        * admit.
-        * admit.
-        * apply H4.
-
+    - destruct IHHderiv with ((empty_env <| env; vars ::= p_map_addall_back xargs vargs |>))...
+        * admit. (* need refl env *)
+        * split.
+            + intros. exfalso.  apply (d_sub_d_empty (empty_env <| env; vars ::= p_map_addall_back xargs vargs |>)).
+                now exists v.
+            + intros. exfalso.  apply (d_sub_d_empty (empty_env <| env; vars ::= p_map_addall_back xargs vargs |>).(mstate)). 
+                now exists x.
+        * clear IHHderiv. exists (ev₀' <| env ; vars ::= {{c\Def z}} |> <| mstate := x |>). econstructor...
+            + eapply (List.Forall2_impl (R1:=generic_exp_sem ev) (generic_exp_sem ev₀'))...
+                intros. assert (List.In a eargs) by admit. 
+                eapply weakening_of_expression_semantics_3... split.
+                ++ intros. apply Henv in H8. intros contra. apply H8. simpl. admit.
+                ++ intros. apply Hmem in H8. destruct H8 as [v [Hev Hnotin]]. exists v. split... 
+                    intros contra. apply Hnotin. simpl. admit.
+            + assert (_determinist_exp_eval exp_sem) by admit. 
+            assert (_determinist_stmt_eval exp_sem stmt_sem) by admit. 
+                pose proof (determinist_stmt_eval _ _ _ H7 H6 _ _ _ _ H2 _ H5). now subst. 
+    
     (* pcall *)
-    - repeat eexists. apply S_PCall with b xargs zargs...
-        * admit.
-        *  admit.
+    - destruct IHHderiv with ((empty_env <| env; vars ::= p_map_addall_back xargs vargs |>))...
+        * admit. (* need refl env *)
+        * split.
+            + intros. exfalso.  apply (d_sub_d_empty (empty_env <| env; vars ::= p_map_addall_back xargs vargs |>)).
+                now exists v.
+            + intros. exfalso.  apply (d_sub_d_empty (empty_env <| env; vars ::= p_map_addall_back xargs vargs |>).(mstate)). 
+                now exists x.
+        * clear IHHderiv. exists (ev₀' <| mstate := x |>). econstructor...
+            + eapply (List.Forall2_impl (R1:=generic_exp_sem ev) (generic_exp_sem ev₀'))...
+                intros. assert (List.In a eargs) by admit. 
+                eapply weakening_of_expression_semantics_3... split.
+                ++ intros. apply Henv in H6. intros contra. apply H6. simpl. admit.
+                ++ intros. apply Hmem in H6. destruct H6 as [v [Hev Hnotin]]. exists v. split... 
+                    intros contra. apply Hnotin. simpl. admit.
 
     (* return *)
     - exists (ev₀' <| env ; vars ::= {{res_f\Def z}} |>). apply S_Return.
         eapply weakening_of_expression_semantics_3 in H...
         
     (* assert *)
-    - exists ev₀'. apply S_PAssert with z... 
-        eapply weakening_of_expression_semantics_3 in H...
-        
+    - exists ev₀'. apply S_PAssert with z...         
 
     (* other cases *)
     - unfold _weakening_of_statement_semantics_3 in ext_stmt_weak.
-        specialize (ext_stmt_weak f  ev (S_Ext s) _ H ev₀' Hrel).
-        destruct ext_stmt_weak as [ev'' Hd]... exists ev''...
+        specialize (ext_stmt_weak f  ev (S_Ext s) _  sub H ev₀' Hrel).
+        destruct ext_stmt_weak as [ev'' Hd]... 
 Admitted.
 
 Definition weakening_of_c_statements_semantics_3 {S T}  := 
     weakening_of_statement_semantics_3 
     (@Empty_exp_sem T) (@Empty_stmt_sem S T) Empty_ext_stmt_vars 
-    (weakening_of_empty_expression_semantics_3 exist_strong_env_mem_partial_order) 
-    (weakening_of_empty_statement_semantics_3 Empty_ext_stmt_vars exist_strong_env_mem_partial_order). 
+    (weakening_of_empty_expression_semantics_3 strong_env_mem_partial_order) 
+    (weakening_of_empty_statement_semantics_3 Empty_ext_stmt_vars strong_env_mem_partial_order). 
