Arithmetic/theories/Languages/Semantics.v
@@ -67,7 +67,7 @@ Definition Forall_routines {F S T } (pgrm : @_c_program F S T)
 Definition well_formed_pgrm (P : fsl_pgrm) (env : Env) (fenv: @fenv _fsl_statement Empty_set) := 
     Forall_routines P ( fun args decls b =>
         (* all used variables are declared *)
-        (forall v, List.In v (fsl_stmt_vars b) -> v ∈ env) /\ 
+        (forall v, StringSet.In v (fsl_stmt_vars b) -> v ∈ env) /\ 
         (* all functions are defined before being called *)
         (forall rvar fname args, 
             @In_stmt _fsl_statement Empty_set (FCall rvar fname args) b -> 
